wordarray: defined mapAccum for update semantics
Defined mapAccum for the update semantics and proved several helper
lemmas about mapAccum which should make proving correspondence between
both the value semantics and the monadic C program easier.

cogent/examples/wa_connect/WordArray_Abstractions.thy
@@ -16,7 +16,6 @@ section "Helper Word Lemmas"
 
 lemma word_mult_cancel_left: 
   fixes a b c :: "('a::len) word"
-  assumes "0 \<le> a" "0 \<le> b" "0 \<le> c"
   assumes "uint c * uint a \<le> uint (max_word :: ('a::len) word)"
   assumes "uint c * uint b \<le> uint (max_word :: ('a::len) word)"
   shows "c * a = c * b \<longleftrightarrow> c = 0 \<or> a = b"
@@ -26,6 +25,19 @@ lemma word_mult_cancel_left:
     apply (clarsimp simp:Abs_word_inject max_word_def uint_word_of_int m1mod2k uint_0_iff )
    apply fastforce
    done
+
+lemma word_mult_cancel_left_bounded: 
+  fixes a b c d :: "('a::len) word"
+  assumes "a \<le> d" "b \<le> d"
+  assumes "unat c * unat d \<le> unat (max_word :: ('a::len) word)"
+  shows "c * a = c * b \<longleftrightarrow> c = 0 \<or> a = b"
+  using assms
+  apply -
+  apply (clarsimp simp: word_le_nat_alt)
+  apply (frule_tac i = "unat a" and j = "unat d" and k = "unat c" in mult_le_mono2)
+  apply (drule_tac i = "unat b" and j = "unat d" and k = "unat c" in mult_le_mono2)
+  by (metis (mono_tags, hide_lams) assms(3) le_unat_uoi mult_left_cancel mult_zero_left not_less_iff_gr_or_eq unat_0 unat_mono word_arith_nat_mult)
+
 
 fun is_prim_type :: "type \<Rightarrow> bool"
   where
@@ -43,6 +55,10 @@ fun size_of_num_type :: "num_type \<Rightarrow> ptrtyp"
 "size_of_num_type U16 = 2" |
 "size_of_num_type U32 = 4" |
 "size_of_num_type U64 = 8"
+
+lemma size_of_num_type_not_zero:
+  "size_of_num_type t \<noteq> 0"
+  by (case_tac t; clarsimp)
 
 fun zero_num_lit :: "num_type \<Rightarrow> lit"
   where
@@ -92,18 +108,11 @@ lemma distinct_indices:
     \<forall>i < len. \<forall>j < len. i = j \<longleftrightarrow> size_of_num_type t * i = size_of_num_type t * j"
   apply clarsimp
   apply (rule iffI)
-   apply (clarsimp simp: wa_abs_typing_u_def)
+   apply clarsimp
   apply (clarsimp simp: wa_abs_typing_u_def)
-  apply (subgoal_tac "0 \<le> i")
-   apply (frule_tac b = j and c = "size_of_num_type t" in word_mult_cancel_left; clarsimp simp: uint_nat)
-     apply (subgoal_tac "int (unat i) < int (unat len)")
-      apply (case_tac t; clarsimp)
-    apply (simp add: unat_mono)
-    apply (subgoal_tac "int (unat j) < int (unat len)")
-     apply (case_tac t; clarsimp)
-    apply (simp add: unat_mono)
-   apply (case_tac t; clarsimp)
-  apply simp
+  apply (cut_tac a = i and b = j and c = "size_of_num_type t" and d = len in word_mult_cancel_left_bounded; simp)
+  apply (erule disjE; clarsimp)
+  apply (case_tac t; clarsimp)
   done      
 end
 
@@ -374,6 +383,12 @@ end
 
 context WordArray begin
 
+subsection "Abbreviations"
+
+abbreviation upd_store :: "('f, 'a, 'l) store \<Rightarrow> 'l \<Rightarrow> ('f, 'a, 'l) uval \<Rightarrow> ('f, 'a, 'l) store"
+  where
+"upd_store \<sigma> p v \<equiv> (\<lambda>l. (if l = p then option.Some v else \<sigma> l))" 
+
 subsection "Level 0 \<xi> Abstractions"
 
 \<comment>\<open> This section contains the abstractions for first order calls to word array functions \<close>
@@ -385,12 +400,14 @@ definition upd_wa_put2_0
   "upd_wa_put2_0 x y =
       (let (x1, x2) = x;
            (y1, y2) = y
-      in (\<exists>p idx val t. x2 = URecord [
+      in (\<exists>p idx val t len arr. x2 = URecord [
           (UPtr p (RCon ''WordArray'' [RPrim (Num t)]), RPtr (RCon ''WordArray'' [RPrim (Num t)])),
           (UPrim (LU32 idx), RPrim (Num U32)), (val, RPrim (Num t))] \<and>
+          x1 p = option.Some (UAbstract (UWA (TPrim (Num t)) len arr)) \<and>
           y2 = UPtr p (RCon ''WordArray'' [RPrim (Num t)]) \<and>
-          y1 = (\<lambda>l. (if \<exists>len arr. x1 p = option.Some (UAbstract (UWA (TPrim (Num t)) len arr)) \<and> 
-                        l = arr + size_of_num_type t * idx \<and> idx < len then option.Some val else x1 l))))"
+          (if idx < len 
+              then y1 = upd_store x1 (arr + size_of_num_type t * idx) val
+              else y1 = x1)))"
 
 definition upd_wa_get_0
   where
@@ -466,6 +483,17 @@ subsection "Level 1 \<xi> Abstractions"
 
 subsubsection "Update Semantics"
 
+lemma valid_ptr_not_in_frame_same:
+  "\<lbrakk>frame \<sigma> w \<sigma>' w'; p \<notin> w; \<sigma> p = option.Some x\<rbrakk> \<Longrightarrow> \<sigma>' p = option.Some x"
+  apply (clarsimp simp: frame_def)
+  apply (erule_tac x = p in allE)
+  apply clarsimp
+  done
+
+lemma frame_single_update:
+  "frame \<sigma> {l} (upd_store \<sigma> l v) {l}"
+  by (clarsimp simp: frame_def)
+
 type_synonym ('f, 'a, 'l) ufoldmapdef = "(char list, atyp, 32 word) uabsfuns \<Rightarrow> ('f, 'a, 'l) store \<Rightarrow> 
                                          32 word \<Rightarrow> 32 word \<Rightarrow> 32 word \<Rightarrow>
                                         'f expr \<Rightarrow> ('f, 'a, 'l) uval \<Rightarrow> ('f, 'a, 'l) uval \<Rightarrow> ptrtyp set\<Rightarrow>
@@ -519,18 +547,14 @@ declare upd_wa_foldnb_bod.simps[simp del]
 lemma upd_wa_foldnb_bod_to_geq_len:
   "\<lbrakk>upd_wa_foldnb_bod \<xi>\<^sub>u \<sigma> p frm len f acc obsv s (\<sigma>', r); \<sigma> p = option.Some (UAbstract (UWA t len arr));
     to \<ge> len\<rbrakk> \<Longrightarrow> upd_wa_foldnb_bod \<xi>\<^sub>u \<sigma> p frm to f acc obsv s (\<sigma>', r)"
-  apply (induct arbitrary: to arr t 
-                rule: upd_wa_foldnb_bod.induct[of _ \<xi>\<^sub>u \<sigma> p frm len f acc obsv s "(\<sigma>', r)"])
+  apply (induct rule: upd_wa_foldnb_bod.induct[of _ \<xi>\<^sub>u \<sigma> p frm to f acc obsv s "(\<sigma>', r)"])
   apply clarsimp
-  apply (drule_tac x = to in meta_spec)
+  apply (drule_tac x = len in meta_spec)
   apply (subst (asm) upd_wa_foldnb_bod.simps)
   apply (clarsimp split: if_splits)
   apply (erule disjE; clarsimp)
    apply (drule_tac x = acc' in meta_spec)
    apply (drule_tac x = \<sigma>' in meta_spec)
-   apply (drule_tac x = toa in meta_spec)
-   apply (drule_tac x = arr in meta_spec)
-   apply (drule_tac x = "TPrim (Num ta)" in meta_spec)
    apply (subst upd_wa_foldnb_bod.simps)
    apply clarsimp
    apply (rule conjI; clarsimp)
@@ -549,9 +573,6 @@ lemma upd_wa_foldnb_bod_to_geq_len:
   apply clarsimp
   apply (drule_tac x = acc' in meta_spec)
   apply (drule_tac x = \<sigma>' in meta_spec)
-  apply (drule_tac x = toa in meta_spec)
-  apply (drule_tac x = arr in meta_spec)
-  apply (drule_tac x = "TPrim (Num ta)" in meta_spec)
   apply clarsimp
   apply (rule_tac x = acc' in exI)
   apply (rule_tac x = \<sigma>' in exI)
@@ -561,8 +582,7 @@ lemma upd_wa_foldnb_bod_to_geq_len:
   apply (rule conjI)
    apply (rule_tac x = x in exI; clarsimp)
   apply (erule meta_mp)
-  apply (clarsimp simp: frame_def)
-  apply (erule_tac x = p in allE; clarsimp)
+  apply (drule_tac p = p in valid_ptr_not_in_frame_same; simp)
   done
 
 lemma upd_wa_foldnb_bod_to_geq_lenD:
@@ -585,8 +605,8 @@ lemma upd_wa_foldnb_bod_to_geq_lenD:
    apply clarsimp
    apply (rule conjI)
     apply (rule_tac x = x in exI; clarsimp)
-   apply (clarsimp simp: frame_def)
-   apply (erule_tac x = p in allE; clarsimp)
+   apply (drule_tac p = p in valid_ptr_not_in_frame_same; simp?)
+   apply (erule meta_impE; simp)
   apply (case_tac "frm < to")
    apply (subst upd_wa_foldnb_bod.simps)
    apply clarsimp
@@ -600,8 +620,8 @@ lemma upd_wa_foldnb_bod_to_geq_lenD:
    apply clarsimp
    apply (rule conjI)
     apply (rule_tac x = x in exI; clarsimp)
-   apply (clarsimp simp: frame_def)
-   apply (erule_tac x = p in allE; clarsimp)
+   apply (drule_tac p = p in valid_ptr_not_in_frame_same; simp?)
+   apply (erule meta_impE; simp)
   apply clarsimp
   apply (subgoal_tac "\<not> frm < len")
    apply (subst upd_wa_foldnb_bod.simps)
@@ -616,7 +636,7 @@ lemma upd_wa_foldnb_bod_step:
     ({p} \<union> s \<union> {arr + size_of_num_type t * i | i. i < len}) \<inter> w1 = {};
     \<xi>\<^sub>u, [URecord [(v, upd.uval_repr v), (r, upd.uval_repr r), (obsv, upd.uval_repr obsv)]] \<turnstile> (\<sigma>', App f (Var 0))\<Down>! (\<sigma>'', r')\<rbrakk> 
     \<Longrightarrow> upd_wa_foldnb_bod \<xi>\<^sub>u \<sigma> p frm (to + 1) f acc obsv s (\<sigma>'', r')"
-  apply (induct arbitrary: len arr v r r' \<sigma>' \<sigma>'' t w1 w2
+  apply (induct arbitrary: r  \<sigma>'
                 rule: upd_wa_foldnb_bod.induct[of _ \<xi>\<^sub>u \<sigma> p frm to f acc obsv s "(\<sigma>', r)"])
   apply clarsimp
   apply (drule_tac x = len in meta_spec)
@@ -624,16 +644,8 @@ lemma upd_wa_foldnb_bod_step:
   apply (clarsimp split: if_splits)
    apply (drule_tac x = acc' in meta_spec)
    apply (drule_tac x = \<sigma>'''' in meta_spec)
-   apply (drule_tac x = len in meta_spec)
-   apply (drule_tac x = arr in meta_spec)
-   apply (drule_tac x = v in meta_spec)
    apply (drule_tac x = b in meta_spec)
-   apply (drule_tac x = r' in meta_spec)
    apply (drule_tac x = a in meta_spec)
-   apply (drule_tac x = \<sigma>'' in meta_spec)
-   apply (drule_tac x = t in meta_spec)
-   apply (drule_tac x = w1 in meta_spec)
-   apply (drule_tac x = w2 in meta_spec)
    apply clarsimp
    apply (subst upd_wa_foldnb_bod.simps)
    apply clarsimp
@@ -647,17 +659,10 @@ lemma upd_wa_foldnb_bod_step:
      apply (rule_tac x = x in exI; clarsimp)
     apply (case_tac "frma + 1 \<le> toa")
      apply clarsimp
-     apply (erule_tac x = toa in allE; clarsimp)
-     apply (thin_tac "frame _ _ _ _")
-     apply (thin_tac "_ = {}")
-     apply (clarsimp simp: frame_def)
-     apply (frule_tac x = pa in spec)
+     apply (frule_tac p = pa and w = w1a in valid_ptr_not_in_frame_same; simp?)
+     apply (frule_tac p = "arr + size_of_num_type t * toa" and w = w1a in valid_ptr_not_in_frame_same; simp?)
+      apply blast
      apply clarsimp
-     apply (erule_tac x = "arr + size_of_num_type t * toa" in allE)
-     apply clarsimp
-     apply (drule_tac x = "arr + size_of_num_type t * toa" in orthD1; simp)
-     apply (rule disjI2)
-     apply (rule_tac x = toa in exI; clarsimp)
     apply (clarsimp simp: not_le)
     apply (drule_tac i = frma and m = toa in inc_le)
     apply (rule FalseE)
@@ -679,16 +684,12 @@ lemma upd_wa_foldnb_bod_step:
     apply (rule_tac x = len in exI)
     apply (rule_tac x = arr in exI)
     apply (rule conjI)
-     apply (clarsimp simp: frame_def)
-     apply (erule_tac x = pa in allE; clarsimp)
+     apply (drule_tac p = pa in valid_ptr_not_in_frame_same; simp)
     apply clarsimp
     apply (erule_tac x = i in allE; clarsimp)
     apply (rule_tac x = va in exI)
-    apply (clarsimp simp: frame_def)
-    apply (erule_tac x = "arr + size_of_num_type t * i" in allE; clarsimp)
-    apply (drule_tac x = "arr + size_of_num_type t * i" in orthD1; simp)
-    apply (rule disjI2)
-    apply (rule_tac x = i in exI; clarsimp)
+    apply (drule_tac p = "arr + size_of_num_type t * i" in valid_ptr_not_in_frame_same; simp?)
+    apply blast
    apply (clarsimp simp: not_less)
    apply (meson less_is_non_zero_p1 word_le_not_less word_overflow)
   apply (clarsimp simp: not_less)
@@ -698,53 +699,28 @@ lemma upd_wa_foldnb_bod_back_step':
   "\<lbrakk>upd_wa_foldnb_bod \<xi>\<^sub>u \<sigma> p frm to f acc obsv s (\<sigma>', r); 
     \<sigma> p = option.Some (UAbstract (UWA t len arr)); len < to\<rbrakk>
     \<Longrightarrow> upd_wa_foldnb_bod \<xi>\<^sub>u \<sigma> p frm (to - 1) f acc obsv s (\<sigma>', r)"
-  apply (induct arbitrary: len arr t
-                rule: upd_wa_foldnb_bod.induct[of _  \<xi>\<^sub>u \<sigma> p frm to f acc obsv s "(\<sigma>', r)"]; clarsimp)
+  apply (induct rule: upd_wa_foldnb_bod.induct[of _  \<xi>\<^sub>u \<sigma> p frm to f acc obsv s "(\<sigma>', r)"]; clarsimp)
   apply (drule_tac x = len in meta_spec)
   apply (erule upd_wa_foldnb_bod.elims)  
   apply (subst upd_wa_foldnb_bod.simps)
   apply (clarsimp split: if_split_asm)
   apply (rule_tac x = ta in exI)
   apply (rule conjI; clarsimp)
-  apply (erule disjE; clarsimp)
-    apply (drule_tac x = acc' in meta_spec)
-    apply (drule_tac x = \<sigma>'' in meta_spec)
-    apply (drule_tac x = len in meta_spec)
-    apply (drule_tac x = arr in meta_spec)
-    apply (drule_tac x = "TPrim (Num ta)" in meta_spec)
-    apply clarsimp
-    apply (rule_tac x = acc' in exI)
-    apply (rule_tac x = \<sigma>'' in exI)
-    apply clarsimp
-    apply (rule_tac x = w1 in exI)
-    apply clarsimp
-    apply (rule conjI)
-     apply (rule_tac x = x in exI; clarsimp)
-    apply (erule meta_mp)
-    apply (clarsimp simp: frame_def)
-    apply (erule_tac x = pa in allE; clarsimp)
-   apply (erule impE)
-   apply simp
+   apply (cut_tac x = frma and n = "toa - 1" in plus_one_helper2; simp)
+    apply auto[1]
    apply clarsimp
    apply (drule_tac x = acc' in meta_spec)
-   apply (drule_tac x = \<sigma>' in meta_spec)
-   apply (drule_tac x = len in meta_spec)
-   apply (drule_tac x = arr in meta_spec)
-   apply (drule_tac x = "TPrim (Num ta)" in meta_spec)
+   apply (drule_tac x = \<sigma>'' in meta_spec)
    apply clarsimp
    apply (rule_tac x = acc' in exI)
-   apply (rule_tac x = \<sigma>' in exI)
+   apply (rule_tac x = \<sigma>'' in exI)
    apply clarsimp
    apply (rule_tac x = w1 in exI)
    apply clarsimp
    apply (rule conjI)
     apply (rule_tac x = x in exI; clarsimp)
-   apply (erule meta_impE)
-    apply simp
-   apply (erule meta_impE)
-    apply (clarsimp simp: frame_def)
-    apply (erule_tac x = pa in allE; clarsimp)
-   apply simp
+   apply (erule meta_mp)
+   apply (drule_tac p = pa in valid_ptr_not_in_frame_same; simp)
   apply (rule FalseE)
   by (metis (no_types, hide_lams) less_1_simp word_le_less_eq word_not_le)
 
@@ -756,25 +732,21 @@ lemma upd_wa_foldnb_bod_back_step:
         (\<xi>\<^sub>u, [URecord [(v, upd.uval_repr v), (r'', upd.uval_repr r''), 
           (obsv, upd.uval_repr obsv)]] \<turnstile> (\<sigma>'', App f (Var 0))\<Down>! (\<sigma>', r)) \<and>
         frame \<sigma>'' w1 \<sigma>' w2 \<and> ({p} \<union> s \<union> {arr + size_of_num_type t * i | i. i < len}) \<inter> w1 = {}"
-  apply (induct arbitrary: len arr \<sigma>' r t
+  apply (induct arbitrary: \<sigma>' r
                 rule: upd_wa_foldnb_bod.induct[of _ \<xi>\<^sub>u \<sigma> p frm to f acc obsv s "(\<sigma>', r)"]; clarsimp)
   apply (erule upd_wa_foldnb_bod.elims)  
   apply (clarsimp split: if_split_asm)
    apply (drule_tac x = len in meta_spec)
    apply (drule_tac x = acc' in meta_spec)
    apply (drule_tac x = \<sigma>''' in meta_spec)
-   apply (drule_tac x = len in meta_spec)
-   apply (drule_tac x = arr in meta_spec)
    apply (drule_tac x = a in meta_spec)
    apply (drule_tac x = b in meta_spec)
-   apply (drule_tac x = t in meta_spec)
    apply clarsimp
    apply (case_tac "frma < to"; clarsimp)
     apply (drule meta_mp)
      apply (metis (no_types, hide_lams) add.commute inc_le plus_le_left_cancel_wrap word_le_less_eq word_le_not_less word_plus_strict_mono_right)
     apply (drule meta_mp)
-     apply (clarsimp simp: frame_def)
-     apply (erule_tac x = pa in allE; clarsimp)
+     apply (drule_tac p = pa in valid_ptr_not_in_frame_same; simp)
     apply clarsimp
     apply (rule_tac x = \<sigma>'''' in exI)
     apply (rule_tac x = r'' in exI)
@@ -794,9 +766,7 @@ lemma upd_wa_foldnb_bod_back_step:
      apply (metis (no_types, hide_lams) add.commute less_is_non_zero_p1 plus_one_helper plus_one_helper2 word_neq_0_conv word_not_le)
     apply (rule_tac x = va in exI)
     apply clarsimp
-    apply (subst (asm) frame_def)
-    apply (erule_tac x = "arr + size_of_num_type t * to" in allE)
-    apply clarsimp
+    apply (drule_tac p = "arr + size_of_num_type t * to" in valid_ptr_not_in_frame_same; simp; clarsimp)
     apply (drule_tac x = "arr + size_of_num_type t * to" in orthD1; simp)
     apply (rule disjI2)
     apply (rule_tac x = to in exI)
@@ -814,6 +784,321 @@ lemma upd_wa_foldnb_bod_back_step:
   apply (rule FalseE)
   by auto
 
+function upd_wa_mapAccumnb_bod :: "(char list, atyp, ptrtyp) ufoldmapdef"
+  where
+  "upd_wa_mapAccumnb_bod \<xi>\<^sub>u \<sigma> p frm to f acc obsv s res = (\<exists>t len arr. 
+    \<sigma> p = option.Some (UAbstract (UWA (TPrim (Num t)) len arr)) \<and> 
+    (\<forall>i<len. \<exists>v. \<sigma> (arr + size_of_num_type t * i) = option.Some v) \<and>
+    (\<forall>i<len. p \<noteq> (arr + size_of_num_type t * i)) \<and>
+    (if frm < min to len then 
+      (\<exists>v v' acc' \<sigma>' w1 w2. \<sigma> (arr + size_of_num_type t * frm) = option.Some v \<and>
+      (\<xi>\<^sub>u, [(URecord [(v, upd.uval_repr v), (acc, upd.uval_repr acc), (obsv, upd.uval_repr obsv)])]
+        \<turnstile> (\<sigma>, App f (Var 0)) \<Down>! (\<sigma>', URecord [ (v', upd.uval_repr v'), (acc', upd.uval_repr acc')])) \<and>
+      frame \<sigma> w1 \<sigma>' w2 \<and> ({p} \<union> s \<union> {arr + size_of_num_type t * i | i. i < len}) \<inter> w1 = {} \<and>
+      upd_wa_mapAccumnb_bod \<xi>\<^sub>u (upd_store \<sigma>'(arr + size_of_num_type t * frm) v') p (frm + 1) to f 
+        acc' obsv s res) 
+    else res = (\<sigma>, URecord [
+      (UPtr p (RCon ''WordArray'' [RPrim (Num t)]), RPtr (RCon ''WordArray'' [RPrim (Num t)])), 
+      (acc, upd.uval_repr acc)])))"
+  by pat_completeness auto
+termination
+  apply (relation "measure (\<lambda>(_, _, _, frm, to, _, _, _, _,  _). unat to - unat frm)"; clarsimp)
+  apply (clarsimp simp: word_less_nat_alt)
+  apply (cut_tac n = frm in unat_Suc2; clarsimp)
+   apply (cut_tac y = to in word_not_simps(3); clarsimp simp: word_less_nat_alt)
+  apply linarith
+  done
+
+declare upd_wa_mapAccumnb_bod.simps[simp del]
+
+lemma upd_wa_mapAccumnb_bod_to_geq_len:
+  "\<lbrakk>upd_wa_mapAccumnb_bod \<xi>\<^sub>u \<sigma> p frm len f acc obsv s (\<sigma>', r); \<sigma> p = option.Some (UAbstract (UWA t len arr));
+    to \<ge> len\<rbrakk> \<Longrightarrow> upd_wa_mapAccumnb_bod \<xi>\<^sub>u \<sigma> p frm to f acc obsv s (\<sigma>', r)"
+  apply (induct rule: upd_wa_mapAccumnb_bod.induct[of _ \<xi>\<^sub>u \<sigma> p frm to f acc obsv s "(\<sigma>', r)"])
+  apply clarsimp
+  apply (case_tac "frm \<ge> len")
+   apply (erule upd_wa_mapAccumnb_bod.elims; clarsimp split: if_splits)
+   apply (drule_tac x = frma in leD; clarsimp)
+   apply (subst upd_wa_mapAccumnb_bod.simps; clarsimp)
+  apply (erule upd_wa_mapAccumnb_bod.elims)
+  apply (clarsimp split: if_split_asm)
+  apply (drule_tac x = frma in not_le_imp_less; clarsimp)
+  apply (drule_tac x = ta in meta_spec)
+  apply (drule_tac x = len in meta_spec)
+  apply (drule_tac x = arr in meta_spec)
+  apply (drule_tac x = v' in meta_spec)
+  apply (drule_tac x = acc' in meta_spec)
+  apply (drule_tac x = \<sigma>'' in meta_spec)
+  apply clarsimp
+  apply (drule meta_mp)
+   apply (drule_tac c = to in order.strict_trans2; simp)
+  apply (subst upd_wa_mapAccumnb_bod.simps; clarsimp)
+  apply (frule_tac c = to in order.strict_trans2; simp)
+  apply (rule_tac x = v' in exI)
+  apply (rule_tac x = acc' in exI)
+  apply (rule_tac x = \<sigma>'' in exI)
+  apply clarsimp
+  apply (rule_tac x = w1 in exI)
+  apply clarsimp
+  apply (rule conjI)
+   apply (rule_tac x = x in exI)
+   apply clarsimp
+  apply (erule meta_impE; simp?)
+  apply (drule_tac p = pa in valid_ptr_not_in_frame_same; simp)
+  done
+
+lemma upd_wa_mapAccumnb_bod_to_geq_lenD:
+  "\<lbrakk>upd_wa_mapAccumnb_bod \<xi>\<^sub>u \<sigma> p frm to f acc obsv s (\<sigma>', r); \<sigma> p = option.Some (UAbstract (UWA t len arr));
+    to \<ge> len\<rbrakk> \<Longrightarrow> upd_wa_mapAccumnb_bod \<xi>\<^sub>u \<sigma> p frm len f acc obsv s (\<sigma>', r)"
+  apply (induct rule: upd_wa_mapAccumnb_bod.induct[of _ \<xi>\<^sub>u \<sigma> p frm to f acc obsv s "(\<sigma>', r)"])
+  apply clarsimp
+ apply (case_tac "frm \<ge> len")
+   apply (erule upd_wa_mapAccumnb_bod.elims; clarsimp split: if_splits)
+   apply (drule_tac x = frma in leD; clarsimp)
+   apply (subst upd_wa_mapAccumnb_bod.simps; clarsimp)
+  apply (erule upd_wa_mapAccumnb_bod.elims)
+  apply (clarsimp split: if_split_asm)
+  apply (drule_tac x = frma in not_le_imp_less; clarsimp)
+  apply (frule_tac c = toa in order.strict_trans2; clarsimp)
+  apply (drule_tac x = ta in meta_spec)
+  apply (drule_tac x = len in meta_spec)
+  apply (drule_tac x = arr in meta_spec)
+  apply (drule_tac x = v' in meta_spec)
+  apply (drule_tac x = acc' in meta_spec)
+  apply (drule_tac x = \<sigma>'' in meta_spec)
+  apply clarsimp
+  apply (subst upd_wa_mapAccumnb_bod.simps; clarsimp)
+  apply (rule_tac x = v' in exI)
+  apply (rule_tac x = acc' in exI)
+  apply (rule_tac x = \<sigma>'' in exI)
+  apply clarsimp
+  apply (rule_tac x = w1 in exI)
+  apply clarsimp
+  apply (rule conjI)
+   apply (rule_tac x = x in exI)
+   apply clarsimp
+  apply (erule meta_impE; simp?)
+  apply (drule_tac p = pa in valid_ptr_not_in_frame_same; simp)
+  done
+
+lemma upd_wa_mapAccumnb_bod_preservation':
+  "\<lbrakk>upd_wa_mapAccumnb_bod \<xi>\<^sub>u \<sigma> p frm to f acc obsv s r; \<sigma> p = option.Some (UAbstract (UWA t len arr))\<rbrakk>
+    \<Longrightarrow> \<exists>\<sigma>' racc. r = (\<sigma>', URecord [
+      (UPtr p (RCon ''WordArray'' [type_repr t]), RPtr (RCon ''WordArray'' [type_repr t])),
+      (racc, upd.uval_repr racc)])"
+  apply (induct rule: upd_wa_mapAccumnb_bod.induct[of _ \<xi>\<^sub>u \<sigma> p frm to f acc obsv s r])
+  apply (erule upd_wa_mapAccumnb_bod.elims; clarsimp split: if_splits)
+  apply (erule disjE; clarsimp)
+  apply (drule_tac x = ta in meta_spec)
+  apply (drule_tac x = len in meta_spec)
+  apply (drule_tac x = arr in meta_spec)
+  apply (drule_tac x = v' in meta_spec)
+  apply (drule_tac x = acc' in meta_spec)
+  apply (drule_tac x = \<sigma>'' in meta_spec)
+  apply clarsimp
+  apply (drule_tac p = pa in valid_ptr_not_in_frame_same; simp?)
+  apply clarsimp
+  done
+
+lemma upd_wa_mapAccumnb_bod_step:
+  "\<lbrakk>upd_wa_mapAccumnb_bod \<xi>\<^sub>u \<sigma> p frm to f acc obsv s (\<sigma>', URecord [rp, (r, upd.uval_repr r)]); 
+    \<sigma> p = option.Some (UAbstract (UWA (TPrim (Num t)) len arr)); frm \<le> to; to < len;
+    unat (size_of_num_type t) * unat len \<le> unat (max_word :: ptrtyp);
+    \<sigma> (arr + size_of_num_type t * to) = option.Some v; frame \<sigma>' w1 \<sigma>'' w2; 
+    ({p} \<union> s \<union> {arr + size_of_num_type t * i | i. i < len}) \<inter> w1 = {};
+    \<xi>\<^sub>u, [URecord [(v, upd.uval_repr v), (r, upd.uval_repr r), (obsv, upd.uval_repr obsv)]] \<turnstile> 
+      (\<sigma>', App f (Var 0))\<Down>! (\<sigma>'', URecord [ (v', upd.uval_repr v'), (r', upd.uval_repr r')])\<rbrakk> 
+    \<Longrightarrow> upd_wa_mapAccumnb_bod \<xi>\<^sub>u \<sigma> p frm (to + 1) f acc obsv s 
+      (upd_store \<sigma>'' (arr + size_of_num_type t * to) v', URecord [rp, (r', upd.uval_repr r')])"
+  apply (induct arbitrary: r \<sigma>'
+                rule: upd_wa_mapAccumnb_bod.induct[of _ \<xi>\<^sub>u \<sigma> p frm to f acc obsv s "(\<sigma>', URecord [rp, (r, upd.uval_repr r)])"])
+  apply clarsimp
+  apply (drule_tac x = t in meta_spec)
+  apply (drule_tac x = len in meta_spec)
+  apply (drule_tac x = arr in meta_spec)
+  apply (erule upd_wa_mapAccumnb_bod.elims; clarsimp split: if_splits)
+   apply (drule_tac x = v'a in meta_spec)
+   apply (drule_tac x = acc' in meta_spec)
+   apply (drule_tac x = \<sigma>'''' in meta_spec)
+   apply (drule_tac x = r in meta_spec)
+   apply (drule_tac x = a in meta_spec)
+   apply (subst upd_wa_mapAccumnb_bod.simps; clarsimp)
+   apply (rule conjI; clarsimp)
+    apply (rule_tac x = v'a in exI)
+    apply (rule_tac x = acc' in exI)
+    apply (rule_tac x = \<sigma>'''' in exI)
+    apply clarsimp
+    apply (rule_tac x = w1a in exI)
+    apply clarsimp
+    apply (rule conjI)
+     apply (rule_tac x = x in exI)
+     apply clarsimp
+    apply (drule meta_mp)
+     apply (drule_tac p = pa and w = w1a in valid_ptr_not_in_frame_same; simp)
+    apply (drule meta_mp)
+     apply (simp add: inc_le)
+    apply (drule meta_mp; simp)
+    apply (rule conjI; clarsimp)
+     apply (drule_tac a = frma and b = toa in word_mult_cancel_left_bounded[rotated 2]; simp)
+     apply (erule disjE)
+      apply (case_tac t; clarsimp)
+     apply (rule FalseE)
+     apply blast
+    apply (drule_tac p = "arr + size_of_num_type t * toa" and w = w1a in valid_ptr_not_in_frame_same; simp)
+    apply blast
+   apply (rule FalseE)
+   apply (simp add: less_is_non_zero_p1 plus_one_helper2)
+  apply (subst upd_wa_mapAccumnb_bod.simps; clarsimp)
+  apply (rule conjI; clarsimp)
+   apply (rule_tac x = v' in exI)
+   apply (rule_tac x = r' in exI)
+   apply (rule_tac x = \<sigma>'' in exI)
+   apply clarsimp
+   apply (rule_tac x = w1 in exI)
+   apply clarsimp
+   apply (rule conjI)
+    apply (rule_tac x = w2 in exI)
+    apply clarsimp
+   apply (subst upd_wa_mapAccumnb_bod.simps; clarsimp)
+   apply (rule_tac x = len in exI)
+   apply (rule_tac x = arr in exI)
+   apply clarsimp
+   apply (rule conjI)
+    apply (drule_tac p = pa in valid_ptr_not_in_frame_same; simp)
+   apply clarsimp
+   apply (erule_tac x = i in allE)
+   apply clarsimp
+   apply (rule_tac x = va in exI)
+   apply (drule_tac p = "arr + size_of_num_type t * i" in valid_ptr_not_in_frame_same; simp?)
+   apply blast
+  apply (erule impE)
+   apply (metis (no_types, hide_lams) add.commute dual_order.strict_trans less_le max_word_max word_Suc_le word_le_less_eq word_not_le)
+  apply (rule FalseE)
+  apply clarsimp
+  by auto
+
+lemma upd_wa_mapAccumnb_bod_back_step':
+  "\<lbrakk>upd_wa_mapAccumnb_bod \<xi>\<^sub>u \<sigma> p frm to f acc obsv s (\<sigma>', r); 
+    \<sigma> p = option.Some (UAbstract (UWA t len arr)); len < to\<rbrakk>
+    \<Longrightarrow> upd_wa_mapAccumnb_bod \<xi>\<^sub>u \<sigma> p frm (to - 1) f acc obsv s (\<sigma>', r)"
+  apply (induct rule: upd_wa_mapAccumnb_bod.induct[of _  \<xi>\<^sub>u \<sigma> p frm to f acc obsv s "(\<sigma>', r)"]; clarsimp)
+  apply (erule upd_wa_mapAccumnb_bod.elims)
+  apply (subst upd_wa_mapAccumnb_bod.simps)
+  apply (clarsimp split: if_split_asm)
+  apply (rule_tac x = ta in exI)
+  apply (drule_tac x = ta in meta_spec)
+  apply (drule_tac x = len in meta_spec)
+  apply (drule_tac x = arr in meta_spec)
+  apply (rule conjI; clarsimp)
+   apply (cut_tac x = frma and n = "toa - 1" in plus_one_helper2; simp)
+    apply auto[1]
+   apply clarsimp
+   apply (drule_tac x = v' in meta_spec)
+   apply (drule_tac x = acc' in meta_spec)
+   apply (drule_tac x = \<sigma>'' in meta_spec)
+   apply (frule_tac p = pa in valid_ptr_not_in_frame_same; simp)
+   apply clarsimp
+   apply (rule_tac x = v' in exI)
+   apply (rule_tac x = acc' in exI)
+   apply (rule_tac x = \<sigma>'' in exI)
+   apply clarsimp
+   apply (rule_tac x = w1 in exI)
+   apply clarsimp
+   apply (rule_tac x = x in exI; clarsimp)
+  apply (rule FalseE)
+  apply (metis (no_types, hide_lams) not_less_iff_gr_or_eq word_less_cases)
+  done
+
+lemma upd_wa_mapAccumnb_bod_back_step:
+  "\<lbrakk>upd_wa_mapAccumnb_bod \<xi>\<^sub>u \<sigma> p frm (1 + to) f acc obsv s (\<sigma>', URecord [rp, (r, upd.uval_repr r)]);
+    unat (size_of_num_type t) * unat len \<le> unat (max_word :: ptrtyp);
+    1 + to \<le> len; frm < 1 + to; \<sigma> p = option.Some (UAbstract (UWA (TPrim (Num t)) len arr))\<rbrakk>
+    \<Longrightarrow> \<exists>\<sigma>'' \<sigma>''' r'' w1 w2 v v'.
+      upd_wa_mapAccumnb_bod \<xi>\<^sub>u \<sigma> p frm to f acc obsv s (\<sigma>'', URecord [rp, (r'', upd.uval_repr r'')]) \<and>
+      \<sigma> (arr + size_of_num_type t * to) = option.Some v \<and>
+      (\<xi>\<^sub>u, [URecord [(v, upd.uval_repr v), (r'', upd.uval_repr r''), (obsv, upd.uval_repr obsv)]] 
+        \<turnstile> (\<sigma>'', App f (Var 0))\<Down>! (\<sigma>''', URecord [(v', upd.uval_repr v'), (r, upd.uval_repr r)])) \<and> 
+      \<sigma>' = upd_store \<sigma>''' (arr + size_of_num_type t * to) v' \<and> frame \<sigma>'' w1 \<sigma>''' w2 \<and> 
+      ({p} \<union> s \<union> {arr + size_of_num_type t * i | i. i < len}) \<inter> w1 = {}"
+  apply (induct arbitrary: \<sigma>' r
+                rule: upd_wa_mapAccumnb_bod.induct[of _ \<xi>\<^sub>u \<sigma> p frm to f acc obsv s "(\<sigma>', URecord [rp, (r, upd.uval_repr r)])"]; clarsimp)
+  apply (erule upd_wa_mapAccumnb_bod.elims)
+  apply (drule_tac x = t in meta_spec)
+  apply (drule_tac x = len in meta_spec)
+  apply (drule_tac x = arr in meta_spec)
+  apply (clarsimp split: if_split_asm)
+   apply (drule_tac x = v' in meta_spec)
+   apply (drule_tac x = acc' in meta_spec)
+   apply (drule_tac x = \<sigma>''' in meta_spec)
+   apply (drule_tac x = a in meta_spec)
+   apply (drule_tac x = r in meta_spec)
+   apply clarsimp
+   apply (case_tac "frma < to"; clarsimp)
+    apply (drule meta_mp)
+     apply (metis (no_types, hide_lams) add.commute inc_le plus_le_left_cancel_wrap word_le_less_eq word_le_not_less word_plus_strict_mono_right)
+    apply (drule meta_mp)
+     apply (drule_tac p = pa in valid_ptr_not_in_frame_same; simp)
+    apply clarsimp
+    apply (rule_tac x = \<sigma>'''' in exI)
+    apply (rule_tac x = \<sigma>''''' in exI)
+    apply (rule_tac x = r'' in exI)
+    apply (rule conjI)
+     apply (subst upd_wa_mapAccumnb_bod.simps; clarsimp)
+     apply (rule_tac x = v' in exI)
+     apply (rule_tac x = acc' in exI)
+     apply (rule_tac x = \<sigma>''' in exI)
+     apply clarsimp
+     apply (rule_tac x = w1 in exI)
+     apply clarsimp
+     apply (rule_tac x = x in exI)
+     apply clarsimp
+    apply (rule_tac x = w1a in exI)
+    apply (rule_tac x = w2 in exI)
+    apply (rule_tac x = va in exI)
+    apply clarsimp
+    apply (rule conjI)
+     apply (clarsimp split: if_splits)
+     apply (drule_tac a = frma and b = to in word_mult_cancel_left_bounded[rotated 2]; simp?)
+       apply (metis (no_types, hide_lams) add.commute less_imp_le plus_one_helper2 word_not_le word_not_simps(1))
+      apply (erule disjE)
+       apply (case_tac t; clarsimp)
+      apply (rule FalseE)
+      apply blast
+     apply (erule_tac x = to in allE)
+     apply (erule impE)
+      apply (metis (no_types) add.commute plus_one_helper2 word_not_le word_not_simps(1))
+     apply clarsimp
+     apply (drule_tac p = "arr + size_of_num_type t * to" and w = w1 in valid_ptr_not_in_frame_same; simp)
+      apply (drule_tac x = "arr + size_of_num_type t * to"  and S' = w1 in orthD1; simp)
+      apply (rule disjI2)
+      apply (rule_tac x = to in exI)
+      apply clarsimp
+      apply (metis (no_types) add.commute plus_one_helper2 word_not_le word_not_simps(1))
+     apply clarsimp
+    apply (rule_tac x = v'a in exI)
+    apply clarsimp
+   apply (rule_tac x = \<sigma>'' in exI)
+   apply (rule_tac x = \<sigma>''' in exI)
+   apply (rule_tac x = acca in exI)
+   apply (subst upd_wa_mapAccumnb_bod.simps; clarsimp)
+   apply (frule_tac p = pa in valid_ptr_not_in_frame_same; simp?)
+   apply (rule conjI)
+    apply (frule_tac t = "(TPrim (Num t))" and len = len and arr = arr 
+      in upd_wa_mapAccumnb_bod_preservation'; simp?)
+   apply (rule_tac x = w1 in exI)
+   apply (rule_tac x = x in exI)
+   apply (rule_tac x = v in exI)
+   apply clarsimp
+   apply (rule conjI)
+    apply (drule linorder_class.antisym_conv1)
+    apply (cut_tac x = frma and n = to in plus_one_helper; simp add: add.commute)
+   apply (rule_tac x = v' in exI)
+   apply (subgoal_tac "frma = to")
+    apply (erule upd_wa_mapAccumnb_bod.elims)
+    apply (clarsimp simp: add.commute)
+   apply (metis (mono_tags, hide_lams) add.commute not_less_iff_gr_or_eq plus_one_helper word_le_not_less)
+  apply (rule FalseE)
+  by auto
 
 fun is_uval_fun :: "('f, 'a, 'l) uval \<Rightarrow> bool"
   where
